Set default goal selector to none in SafeReduce and Conversion

safechecker/theories/PCUICSafeConversion.v
@@ -16,6 +16,8 @@ From Equations Require Import Equations.
 Require Import Equations.Prop.DepElim.
 Local Set Keyed Unification.
 
+Set Default Goal Selector "!".
+
 Import MonadNotation.
 
 Module PSR := PCUICSafeReduce.
@@ -28,62 +30,72 @@ Module PSR := PCUICSafeReduce.
  *)
 
 
-Definition wf_global_uctx_invariants {cf:checker_flags} Σ
-  : ∥ wf Σ ∥ -> global_uctx_invariants (global_uctx Σ).
+Definition wf_global_uctx_invariants {cf:checker_flags} Σ :
+  ∥ wf Σ ∥ ->
+  global_uctx_invariants (global_uctx Σ).
 Proof.
   intros [HΣ]. split.
   - cbn. unfold global_levels.
     cut (LevelSet.In lSet (LevelSet_pair Level.lSet Level.lProp)).
     + generalize (LevelSet_pair Level.lSet Level.lProp).
-      clear HΣ. induction Σ; simpl. easy.
+      clear HΣ. induction Σ; simpl. 1: easy.
       intros X H. apply LevelSet.union_spec. now right.
     + apply LevelSet.add_spec. right. now apply LevelSet.singleton_spec.
   - unfold global_uctx.
     simpl. intros [[l ct] l'] Hctr. simpl in *.
     induction Σ in HΣ, l, ct, l', Hctr |- *.
-    * apply ConstraintSetFact.empty_iff in Hctr; contradiction.
-    * simpl in *. apply ConstraintSet.union_spec in Hctr;
-                    destruct Hctr as [Hctr|Hctr].
-      -- split.
-         inversion HΣ; subst.
-         destruct H2 as [HH1 [HH HH3]].
-         subst udecl. destruct a as [kn decl|kn decl]; simpl in *.
-         destruct decl; simpl in *.
-         destruct cst_universes;
-           [eapply (HH (l, ct, l') Hctr)|
-            apply ConstraintSetFact.empty_iff in Hctr; contradiction|
-            apply ConstraintSetFact.empty_iff in Hctr; contradiction].
-         destruct decl; simpl in *.
-         destruct ind_universes;
-           [eapply (HH (l, ct, l') Hctr)|
-            apply ConstraintSetFact.empty_iff in Hctr; contradiction|
-            apply ConstraintSetFact.empty_iff in Hctr; contradiction].
-         inversion HΣ; subst.
-         destruct H2 as [HH1 [HH HH3]].
-         subst udecl. destruct a as [kn decl|kn decl]; simpl in *.
-         destruct decl; simpl in *.
-         destruct cst_universes;
-           [eapply (HH (l, ct, l') Hctr)|
-            apply ConstraintSetFact.empty_iff in Hctr; contradiction|
-            apply ConstraintSetFact.empty_iff in Hctr; contradiction].
-         destruct decl; simpl in *.
-         destruct ind_universes;
-           [eapply (HH (l, ct, l') Hctr)|
-            apply ConstraintSetFact.empty_iff in Hctr; contradiction|
-            apply ConstraintSetFact.empty_iff in Hctr; contradiction].
-      -- inversion HΣ; subst.
-         split; apply LevelSet.union_spec; right;
-           unshelve eapply (IHΣ _ _ _ _ Hctr); tea.
+    + apply ConstraintSetFact.empty_iff in Hctr; contradiction.
+    + simpl in *. apply ConstraintSet.union_spec in Hctr.
+      destruct Hctr as [Hctr|Hctr].
+      * split.
+        -- inversion HΣ; subst.
+           destruct H2 as [HH1 [HH HH3]].
+           subst udecl. destruct a as [kn decl|kn decl]; simpl in *.
+           ++ destruct decl; simpl in *.
+              destruct cst_universes ; [
+                eapply (HH (l, ct, l') Hctr)
+              | apply ConstraintSetFact.empty_iff in Hctr ; contradiction
+              | apply ConstraintSetFact.empty_iff in Hctr; contradiction
+              ].
+           ++ destruct decl. simpl in *.
+              destruct ind_universes ; [
+                eapply (HH (l, ct, l') Hctr)
+              | apply ConstraintSetFact.empty_iff in Hctr; contradiction
+              | apply ConstraintSetFact.empty_iff in Hctr; contradiction
+              ].
+        -- inversion HΣ. subst.
+           destruct H2 as [HH1 [HH HH3]].
+           subst udecl. destruct a as [kn decl|kn decl].
+           all: simpl in *.
+           ++ destruct decl. simpl in *.
+              destruct cst_universes ; [
+                eapply (HH (l, ct, l') Hctr)
+              | apply ConstraintSetFact.empty_iff in Hctr; contradiction
+              | apply ConstraintSetFact.empty_iff in Hctr; contradiction
+              ].
+           ++ destruct decl. simpl in *.
+              destruct ind_universes; [
+                eapply (HH (l, ct, l') Hctr)
+              | apply ConstraintSetFact.empty_iff in Hctr; contradiction
+              | apply ConstraintSetFact.empty_iff in Hctr; contradiction
+              ].
+      * inversion HΣ. subst.
+        split.
+        all: apply LevelSet.union_spec.
+        all: right.
+        all: unshelve eapply (IHΣ _ _ _ _ Hctr).
+        all: try eassumption.
 Qed.
 
-Definition wf_ext_global_uctx_invariants {cf:checker_flags} Σ
-  : ∥ wf_ext Σ ∥ -> global_uctx_invariants (global_ext_uctx Σ).
+Definition wf_ext_global_uctx_invariants {cf:checker_flags} Σ :
+  ∥ wf_ext Σ ∥ ->
+  global_uctx_invariants (global_ext_uctx Σ).
 Proof.
   intros [HΣ]. split.
   - apply LevelSet.union_spec. right. unfold global_levels.
     cut (LevelSet.In lSet (LevelSet_pair Level.lSet Level.lProp)).
     + generalize (LevelSet_pair Level.lSet Level.lProp).
-      induction Σ.1; simpl. easy.
+      induction Σ.1; simpl. 1: easy.
       intros X H. apply LevelSet.union_spec. now right.
     + apply LevelSet.add_spec. right. now apply LevelSet.singleton_spec.
   - destruct Σ as [Σ φ]. destruct HΣ as [HΣ Hφ].
@@ -195,7 +207,7 @@ Section Conversion.
   Proof.
     intros Γ [u hu].
     destruct hΣ as [hΣ'].
-    apply normalisation_upto in hu as h.
+    apply normalisation_upto in hu as h. 2: assumption.
     dependent induction h.
     constructor. intros [y hy] r.
     unfold wcored in r. cbn in r.
@@ -513,12 +525,16 @@ Section Conversion.
   Proof.
     pose proof hΣ'.
     apply eqb_term_upto_univ_impl.
-    intros u1 u2; eapply (check_eqb_universe_spec G (global_ext_uctx Σ)); tas.
-    now eapply wf_ext_global_uctx_invariants.
-    now eapply global_ext_uctx_consistent.
-    intros u1 u2; eapply (check_leqb_universe_spec G (global_ext_uctx Σ)); tas.
-    now eapply wf_ext_global_uctx_invariants.
-    now eapply global_ext_uctx_consistent.
+    - intros u1 u2.
+      eapply (check_eqb_universe_spec G (global_ext_uctx Σ)).
+      + now eapply wf_ext_global_uctx_invariants.
+      + now eapply global_ext_uctx_consistent.
+      + assumption.
+    - intros u1 u2.
+      eapply (check_leqb_universe_spec G (global_ext_uctx Σ)).
+      + now eapply wf_ext_global_uctx_invariants.
+      + now eapply global_ext_uctx_consistent.
+      + assumption.
   Qed.
 
   Lemma eqb_term_spec t u :
@@ -527,12 +543,16 @@ Section Conversion.
   Proof.
     pose proof hΣ'.
     apply eqb_term_upto_univ_impl.
-    intros u1 u2; eapply (check_eqb_universe_spec G (global_ext_uctx Σ)); tas.
-    now eapply wf_ext_global_uctx_invariants.
-    now eapply global_ext_uctx_consistent.
-    intros u1 u2; eapply (check_eqb_universe_spec G (global_ext_uctx Σ)); tas.
-    now eapply wf_ext_global_uctx_invariants.
-    now eapply global_ext_uctx_consistent.
+    - intros u1 u2.
+      eapply (check_eqb_universe_spec G (global_ext_uctx Σ)).
+      + now eapply wf_ext_global_uctx_invariants.
+      + now eapply global_ext_uctx_consistent.
+      + assumption.
+    - intros u1 u2.
+      eapply (check_eqb_universe_spec G (global_ext_uctx Σ)).
+      + now eapply wf_ext_global_uctx_invariants.
+      + now eapply global_ext_uctx_consistent.
+      + assumption.
   Qed.
 
   Lemma eqb_term_refl :
@@ -1395,13 +1415,16 @@ Section Conversion.
     intros []; auto.
   Defined.
 
-  Lemma wellformed_wf_local Γ t : wellformed Σ Γ t -> ∥ wf_local Σ Γ ∥.
+  Lemma wellformed_wf_local Γ t :
+    wellformed Σ Γ t ->
+    ∥ wf_local Σ Γ ∥.
   Proof.
-    intros []. destruct hΣ. destruct H.
-    now constructor; eapply typing_wf_local in X0.
-    destruct H, hΣ. constructor. red in X.
-    destruct X as [ctx [s [eq wf]]].
-    now eapply All_local_env_app in wf.
+    intros [].
+    - destruct hΣ. destruct H.
+      now constructor ; eapply typing_wf_local in X0.
+    - destruct H, hΣ. constructor. red in X.
+      destruct X as [ctx [s [eq wf]]].
+      now eapply All_local_env_app in wf.
   Qed.
 
   Equations(noeqns) unfold_constants (Γ : context) (leq : conv_pb)
